LL1/Proofs/Parser/SafetyNoFuel.v
@@ -1,0 +1,183 @@
+Require Import List.
+Require Import Omega.
+Require Import String.
+Require Import Wf_nat.
+Require Import Lib.Grammar.
+Require Import Lib.ParseTree.
+Require Import Lib.Tactics.
+Require Import LL1.Parser.
+Require Import LL1.ParseTable.
+Require Import LL1.ParseTableGen.
+Require Import LL1.Parser.
+Require Import LL1.Derivation.
+Require Import CompletenessNoFuel.
+Require Import SoundnessNoFuel.
+Import ListNotations.
+Open Scope list_scope.
+
+Definition sa_size (sa : sym_arg) : nat :=
+  match sa with
+  | F_arg _ => 0
+  | G_arg gamma => 1 + List.length gamma
+  end.
+
+Lemma leftrec_conditions :
+  forall g tbl,
+    parse_table_for tbl g
+    -> forall (input : list string)
+              (vis : NtSet.t)
+              (sa : sym_arg),
+      match sa with
+      | F_arg sym =>
+        forall a x vis' input',
+          parse_nf tbl sym input vis a = inl (LeftRec x vis' input')
+          -> (NtSet.In x vis
+              /\ (sym = NT x
+                  \/ nullable_path g (peek input) sym (NT x)))
+             \/ (*(~ NtSet.In x vis *)
+                 exists la, (left_recursive g (NT x) la)
+      | G_arg gamma =>
+        forall a x vis' input',
+          parseForest_nf tbl gamma input vis a = inl (LeftRec x vis' input')
+          -> (exists pre sym suf,
+                 gamma = pre ++ sym :: suf
+                 /\ nullable_gamma g pre
+                 /\ NtSet.In x vis
+                 /\ (sym = NT x
+                     \/ nullable_path g (peek input) sym (NT x)))
+             \/ (*(~ NtSet.In x vis *)
+                 exists la, (left_recursive g (NT x) la)
+      end.
+Proof.
+  intros g tbl Ht input.
+
+  remember (List.length input) as l.
+  generalize dependent input.
+  induction l as [l IHl] using lt_wf_ind.
+  intros input Hl; subst.
+
+  intros vis.
+  remember (NtSet.cardinal (NtSet.diff (fromNtList (nt_keys tbl)) vis)) as card.
+  generalize dependent vis.
+  induction card as [card IHcard] using lt_wf_ind.
+  intros vis Hcard; subst.
+
+  intros sa.
+  remember (sa_size sa) as sz.
+  generalize dependent sa.
+  induction sz as [sz IHsz] using lt_wf_ind.
+  intros sa Hsa; subst.
+  destruct sa.
+
+  - (* sa = F_arg sym *)
+    intros a x vis' input' Hp; destruct a.
+    step.
+    + step; tc.
+      step; tc.
+    + step; tc.
+      destruct s as [gamma Hlk].
+      step.
+      * (* x is in vis *)
+        inv Hp.
+        left; split; auto.
+      *  (* x is not in vis *)
+        step_eq Hpf.
+        -- inv Hp.
+           eapply IHcard with (sa := G_arg gamma) in Hpf; eauto.
+           clear IHl; clear IHsz; clear IHcard.
+           destruct Hpf as [Hex | Hex].
+           ++ destruct Hex as [pre [sym [suf [Hg [Hng [Hin Hrest]]]]]]; subst.
+              rename x into x'; rename n into x.
+              destruct Hrest as [Hin' | Hnin].
+              ** subst.
+                 destruct (NtSetFacts.eq_dec x x').
+                 --- subst.
+                     right.
+                     exists (peek input).
+                     red.
+                     apply Ht in Hlk.
+                     destruct Hlk.
+                     eapply DirectPath with (pre := pre); eauto.
+                 --- left.
+                     split.
+                     +++ ND.fsetdec.
+                     +++ right.
+                         apply Ht in Hlk.
+                         destruct Hlk.
+                         eapply DirectPath; eauto.
+              ** destruct (NtSetFacts.eq_dec x x').
+                 --- subst.
+                     right.
+                     exists (peek input).
+                     red.
+                     destruct sym as [y | z].
+                     +++ inv Hnin.
+                     +++ apply Ht in Hlk; destruct Hlk.
+                         eapply IndirectPath with (y := z); eauto.
+                 --- left.
+                     split.
+                     +++ ND.fsetdec.
+                     +++ right.
+                         destruct sym.
+                         *** inv Hnin.
+                         *** apply Ht in Hlk; destruct Hlk.
+                             eapply IndirectPath with (y := n1); eauto.
+           ++ right; auto.
+           ++ apply NP.subset_cardinal_lt with (x := n); try ND.fsetdec.
+              apply in_A_not_in_B_in_diff; auto.
+              apply in_list_iff_in_fromNtList.
+              eapply pt_lookup_in_nt_keys; eauto.
+        -- step; tc.
+
+  - intros a x vis' input' Hpf; destruct a.
+    step; tc.
+    step_eq Hpf.
+    + (* calling parse on s returns LeftRec *)
+      inv Hpf.
+      eapply IHsz with (sa := F_arg s) (m := sa_size (F_arg s)) in Hpf0; eauto.
+      * destruct Hpf0; auto.
+        left.
+        exists nil; exists s; exists l; split; auto. 
+      * simpl; omega.
+    + (* calling parse on s succeeds, calling parseForest on l returns LeftRec *)
+      step.
+      step.
+      * (* parse consumed some input *)
+        step_eq Hpf.
+        -- inv Hpf.
+           eapply IHl with (sa := G_arg l) in Hpf1; eauto.
+           destruct Hpf1.
+           ++ destruct H as [pre [sym [suf [Heq [Hng [Hin Hrest]]]]]].
+              ND.fsetdec.
+           ++ right; auto.
+        -- step; tc.
+      * (* parse returned a null tree *)
+        step_eq Hpf.
+        -- inv Hpf.
+           pose proof Hpf0 as Hpf0'.
+           eapply input_length_invariant in Hpf0; eauto.
+           destruct Hpf0.
+           ++ contradiction.
+           ++ destruct H; subst.
+              eapply IHsz with (sa := G_arg l) in Hpf1; eauto.
+              destruct Hpf1.
+              ** destruct H0 as [pre [sym [suf [Heq [Hng [Hin Hrest]]]]]]; subst.
+                 left.
+                 exists (s :: pre); exists sym; exists suf.
+                 repeat split; auto.
+              ** right; auto.
+        -- step; tc.
+Qed.
+
+Theorem parse_nf_safe :
+  forall g tbl sym input x vis' input',
+    parse_table_for tbl g
+    -> ~ parse_wrapper tbl sym input = inl (LeftRec x vis' input').
+Proof.
+  intros g tbl sym input s vis' input' Htbl; unfold not; unfold parse_wrapper; intros Hp.
+  eapply leftrec_conditions with (sa := F_arg sym) in Hp; eauto.
+  destruct Hp.
+  - ND.fsetdec.
+  - destruct H as [la Hlr].
+    eapply LL1_parse_table_impl_no_left_recursion; eauto.
+Qed.
